changed visibility of parameters to terms

theories/AlmostStlc/Examples.v
@@ -1,6 +1,10 @@
 Require Export Syntax.
 Require Export Denotation.
 Require Import List.
+From EnTree Require Export 
+     Core.EnTreeDefinition
+     Eq.Eqit
+.
 Import ListNotations.
 From Equations Require Import Equations Signature.
 
@@ -11,7 +15,7 @@ Context {t1 t2 : type}.
 Definition fun_lift : term (Arrow (Arrow t1 MR2 t2) MR3 (Arrow t1 (MR1 ++ MR2) t2 ))
                            Γ MR3.
 apply term_abs. apply term_abs.
-apply term_lift. apply term_app with (t1 := t1).
+apply term_lift. eapply @term_app with (t1 := t1).
 apply term_var. apply VarS. apply VarZ.
 apply term_var. apply VarZ.
 Defined.
@@ -25,35 +29,66 @@ Definition plus_call : call_frame := [(Nat, Arrow Nat [] Nat)].
 
 Definition plus : term (Arrow Nat [] (Arrow Nat [] Nat)) Γ [].
 apply term_abs. apply term_abs.
-apply term_mfix with (R := plus_call) (MR := [plus_call]) (x := VarZ plus_call []).
+apply @term_mfix with (R := plus_call) (MR := [plus_call]) (x := VarZ).
 - apply mfix_bodies_cons.
   + eapply term_match_nat.
     * apply term_var. apply VarZ.
     * apply term_abs. apply term_var. apply VarZ.
-    * eapply term_app with (t1 := Arrow Nat [] Nat).
+    * eapply @term_app with (t1 := Arrow Nat [] Nat).
       {
         apply term_abs. apply term_abs.
-        apply term_app with (t1 := Nat).
-        - apply term_var. apply VarS. apply VarZ.
-        - apply term_succ. apply term_var. apply VarZ.
+        apply @term_app with (t1 := Nat).
+        - exact (term_var (VarS VarZ)).
+        - exact (term_succ (term_var VarZ)).
       }
       {
-        eapply term_call. apply VarZ. apply VarZ. 
-        apply term_var. apply VarZ.
+        exact (term_call VarZ VarZ (term_var VarZ)).
       }
   + apply mfix_bodies_nil.
-- eapply term_app with (t1 := Nat).
-  + apply term_app with (t1 := Arrow Nat [] Nat).
+- eapply @term_app with (t1 := Nat).
+  + apply @term_app with (t1 := Arrow Nat [] Nat).
     * apply @fun_lift with (MR1 := [plus_call]).
-    * eapply term_call.
-      -- apply VarZ.
-      -- apply VarZ.
-      -- apply term_var. apply VarZ.
-  + apply term_var. apply VarS. apply VarZ.
+    * exact (term_call VarZ VarZ (term_var VarZ)).
+  + exact (term_var (VarS VarZ)). 
 Defined.
 
 End plus.
 
+Section plus'.
+
+Context {Γ : ctx} {MR : mfix_ctx}.
+
+Definition plus_call' : call_frame := [(Pair Nat Nat, Nat) ].
+
+Definition plus' : term (Arrow (Pair Nat Nat) MR Nat) Γ MR.
+apply term_abs. 
+eapply @term_mfix with (R := plus_call') (MR := plus_call' :: MR) (x := VarZ).
+- apply mfix_bodies_cons.
+  + eapply term_split.
+    * apply term_var. apply VarZ.
+    * eapply term_match_nat.
+      -- eapply term_var. eapply VarZ.
+      -- eapply term_var. eapply VarS. eapply VarZ.
+      -- apply term_succ. eapply term_call.
+         apply VarZ. apply VarZ.
+         apply term_pair.
+         apply term_var. apply VarZ.
+         apply term_var. apply VarS. apply VarS. apply VarZ.
+  + apply mfix_bodies_nil.
+- eapply term_call. apply VarZ. apply VarZ.
+  apply term_var. apply VarZ.
+Defined.
+End plus'.
+
+Locate bind_ret_l.
+
+Goal denote_term (term_app (@plus' [] []) (term_pair (term_const 1) (term_const 1))) tt ≈ 
+       Ret 2.
+simp denote_term. unfold plus'. simp denote_term. 
+repeat setoid_rewrite bind_ret_l. unfold plus_call'. simp denote_term.
+cbn. simp denote_term. Transparent denote_term. cbn.
+(* setoid_rewrite bind_ret_l.
+ unfold denote_term.  setoid_rewrite @denote_term_equation_15. *)
 Section map_term.
 Context (t1 t2 : type) (MR : mfix_ctx).
 
@@ -79,7 +114,7 @@ Defined.
 
 Definition map : term (Arrow (Arrow t1 MR t2) [] (Arrow (List t1) MR (List t2))) [] [].
 eapply term_abs. eapply term_abs.
-apply term_mfix with (R := map_call) (MR := map_call :: MR) (x := VarZ map_call MR).
+apply @term_mfix with (R := map_call) (MR := map_call :: MR) (x := VarZ).
 - apply mfix_bodies_cons.
   + apply map_body.
   + apply mfix_bodies_nil.
@@ -91,9 +126,12 @@ Defined.
 End map_term.
 
 Goal False.
-set (denote_term _ _ (map Nat Nat []) tt) as e. cbn in e.
-simp denote_term in e.
-Check (denote_term _ _ (map Nat Nat []) tt).
+set (denote_term (map Nat Nat []) tt) as e. cbn in e.
+simp denote_term in e. cbv in e. simp denote_term in e.
+assert (e = EnTree.spin).
+cbv. simp denote_term.
+
+Check (denote_term (map Nat Nat []) tt).
 
 (*
 \(f : t1 =MR=> t2) (l : List t1) ->_MR  mfix (map_rec :: MR) VarZ 
